Core/Protocol.v
@@ -6,170 +6,10 @@ Require Import Eqdep Relations.
 From HTT
 Require Import pred prelude idynamic ordtype pcm finmap unionmap heap.
 From CasperToychain
-Require Import Blockforest.
+Require Import Blockforest Node Casper.
 Set Implicit Arguments.
 Unset Strict Implicit.
 Unset Printing Implicit Defensive.
-
-Definition Address_ordMixin := fin_ordMixin Address.
-Canonical Address_ordType := Eval hnf in OrdType Address Address_ordMixin.
-
-(* ------------------*)
-(* PROTOCOL MESSAGES *)
-(* ------------------*)
-
-Definition peers_t := seq Address.
-
-Inductive Message :=
-| BlockMsg of block
-| TxMsg of Transaction
-| InvMsg of seq Hash
-| GetDataMsg of Hash.
-
-Inductive InternalTransition :=
-  | TxT of Transaction
-  | MintT.
-
-Definition eq_msg a b :=
- match a, b with
-  | BlockMsg bA, BlockMsg bB => (bA == bB)
-  | BlockMsg _, _ => false
-  | TxMsg tA, TxMsg tB => (tA == tB)
-  | TxMsg _, _ => false
-  | InvMsg hA, InvMsg hB => (hA == hB)
-  | InvMsg _, _ => false
-  | GetDataMsg hA, GetDataMsg hB => (hA == hB)
-  | GetDataMsg _, _ => false
- end.
-
-Ltac simple_tactic mb n n' B :=
-  (case: mb=>//[b'|t'|p'|p']; do? [by constructor 2];
-   case B: (n == n'); [by case/eqP:B=><-; constructor 1|constructor 2];
-   case=>E; subst n'; rewrite eqxx in B).
-
-Lemma eq_msgP : Equality.axiom eq_msg.
-Proof.
-move=> ma mb. rewrite/eq_msg.
-case: ma=>[b|t|h|h].
-- case:mb=>////[b'|t'|h'|h']; do? [by constructor 2].
-  case B: (b == b'); [by case/eqP:B=><-; constructor 1|constructor 2].
-  by case=>Z; subst b'; rewrite eqxx in B.
-- case:mb=>////[b'|t'|h'|h']; do? [by constructor 2].
-  case B: (t == t'); [by case/eqP:B=><-; constructor 1|constructor 2].
-  by case=>Z; subst t'; rewrite eqxx in B.
-- case:mb=>////[b'|t'|h'|h']; do? [by constructor 2].
-  case B: (h == h'); [by case/eqP:B=><-; constructor 1|constructor 2].
-  by case=>Z; subst h'; rewrite eqxx in B.
-- case:mb=>////[b'|t'|h'|h']; do? [by constructor 2].
-  case B: (h == h'); [by case/eqP:B=><-; constructor 1|constructor 2].
-  by case=>Z; subst h'; rewrite eqxx in B.
-Qed.
-  
-Canonical Msg_eqMixin := Eval hnf in EqMixin eq_msgP.
-Canonical Msg_eqType := Eval hnf in EqType Message Msg_eqMixin.
-
-Record Packet := mkP {src: Address; dst: Address; msg: Message}.
-
-Definition eq_pkt a b :=
-  ((src a) == (src b)) && ((dst a) == (dst b)) && ((msg a) == (msg b)).
-
-Lemma eq_pktP : Equality.axiom eq_pkt.
-Proof.
-case=>sa da ma [sb] db mb; rewrite/eq_pkt/=.
-case P1: (sa == sb)=>/=; last by constructor 2; case=>/eqP; rewrite P1.
-case P2: (da == db)=>/=; last by constructor 2; case=> _ /eqP; rewrite P2.
-case P3: (ma == mb)=>/=; last by constructor 2; case=> _ _ /eqP; rewrite P3.
-by constructor 1; move/eqP: P1=><-; move/eqP: P2=><-; move/eqP: P3=><-.
-Qed.
-
-Canonical Packet_eqMixin := Eval hnf in EqMixin eq_pktP.
-Canonical Packet_eqType := Eval hnf in EqType Packet Packet_eqMixin.
-
-Definition ToSend := seq Packet.
-Definition emitZero : ToSend := [::].
-Definition emitOne (packet : Packet) : ToSend := [:: packet].
-Definition emitMany (packets : ToSend) := packets.
-
-Definition emitBroadcast (from : Address) (dst : seq Address) (msg : Message) :=
-  [seq (mkP from to msg) | to <- dst].
-
-(* ------------------*)
-(* NODE STATE & CODE *)
-(* ------------------*)
-
-Record State :=
-  Node {
-    id : Address;
-    peers : peers_t;
-    blockTree : Blockforest;
-    txPool : TxPool;
-  }.
-
-Definition Init (n : Address) (peers : seq Address) : State :=
-  Node n peers (#GenesisBlock \\-> GenesisBlock) [::].
-
-Definition procMsg (st: State) (from : Address) (msg: Message) (ts: Timestamp) :=
-    let: Node n prs bt pool := st in
-    match msg with
-    | BlockMsg b =>
-      let: newBt := btExtend bt b in
-      let: newPool := [seq t <- pool | txValid t (btChain newBt)] in
-      let: ownHashes := (keys_of newBt) ++ [seq hashT t | t <- newPool] in
-      pair (Node n prs newBt newPool) (emitBroadcast n prs (InvMsg ownHashes))
-
-    | TxMsg tx =>
-      let: newPool := tpExtend pool bt tx in
-      let: ownHashes := (keys_of bt) ++ [seq hashT t | t <- newPool] in
-      pair (Node n prs bt newPool) (emitBroadcast n prs (InvMsg ownHashes))
-
-    | InvMsg peerHashes =>
-      let: ownHashes := (keys_of bt) ++ [seq hashT t | t <- pool] in
-      let: newH := [seq h <- peerHashes | h \notin ownHashes] in
-      let: gets := [seq mkP n from (GetDataMsg h) | h <- newH] in
-      pair st (emitMany gets)
-
-    | GetDataMsg h =>
-      (* Do not respond to yourself *)
-      if from == n then pair st emitZero else
-      let: matchingBlocks := [seq b <- [:: get_block bt h] | b != GenesisBlock] in
-      match ohead matchingBlocks with
-      | Some b => pair (Node n prs bt pool) (emitOne (mkP n from (BlockMsg b)))
-      | None =>
-        let: matchingTxs := [seq t <- pool | (hashT t) == h] in
-        match ohead matchingTxs with
-        | Some tx =>
-          pair (Node n prs bt pool) (emitOne (mkP n from (TxMsg tx)))
-        | None => pair st emitZero
-        end
-      end
-    end.
-
-Definition procInt (st : State) (tr : InternalTransition) (ts : Timestamp) :=
-    let: Node n prs bt pool := st in
-    match tr with
-    | TxT tx => pair st (emitBroadcast n prs (TxMsg tx))
-
-    (* Assumption: nodes broadcast to themselves as well! => simplifies logic *)
-    | MintT =>
-      let: bc := btChain bt in
-      let: allowedTxs := [seq t <- pool | txValid t bc] in
-      match genProof n bc allowedTxs ts with
-      | Some pf =>
-        if VAF pf ts bc allowedTxs then
-          let: prevBlock := last GenesisBlock bc in
-          let: block := mkB (hashB prevBlock) allowedTxs pf in
-          if tx_valid_block bc block then
-            let: newBt := btExtend bt block in
-            let: newPool := [seq t <- pool | txValid t (btChain newBt)] in
-            let: ownHashes := (keys_of newBt) ++ [seq hashT t | t <- newPool] in
-            pair (Node n prs newBt newPool) (emitBroadcast n prs (BlockMsg block))
-          else
-            pair st emitZero
-        else
-          pair st emitZero
-      | None => pair st emitZero
-      end
-    end.
 
 Definition StateMap := union_map [ordType of Address] State.
 
@@ -347,7 +187,7 @@ Lemma procMsg_valid :
 Proof.
 move=> s1 from  m ts.
 case Msg: m=>[b|||];
-destruct s1; rewrite/procMsg/=; do?by [|move: (btExtendV blockTree0 b)=><-].
+destruct s1; rewrite/procMsg/=; do?by [|move: (btExtendV blockTree b)=><-].
 case:ifP => //=.
 move/eqP => H_neq; case: ifP; move/eqP => //= H_eq H_v.
 by case ohead.
@@ -362,7 +202,7 @@ case Int: t; destruct s1; rewrite/procInt/=; first by [].
 case: (genProof _); last done.
 move=>Pf; case: (VAF _ _ _); last done.
 case tV: (tx_valid_block _ _)=>//.
-by rewrite/blockTree/=; apply btExtendV.
+by rewrite/Node.blockTree/=; apply btExtendV.
 Qed.
 
 Lemma procMsg_validH :
@@ -388,7 +228,7 @@ case Int: t; destruct s1; rewrite/procInt/=; first by [].
 case: (genProof _); last done.
 move=>Pf; case: (VAF _ _ _); last done.
 case tV: (tx_valid_block _ _)=>//.
-by rewrite/blockTree/=; apply btExtendH.
+by rewrite/Node.blockTree/=; apply btExtendH.
 Qed.
 
 Lemma procMsg_has_init_block:
